theories/coroutine.v
@@ -1,0 +1,641 @@
+Require Export refframe.module.
+Require Import refframe.trefines.
+Require Import refframe.filter.
+Require Import refframe.product.
+Require Import refframe.seq_product.
+Require Import refframe.link.
+Require Import refframe.proof_techniques.
+Require Import refframe.prepost.
+Require Import refframe.imp.
+Require Import refframe.asm.
+Require Import refframe.itree.
+Require Import refframe.imp_to_asm.
+Require Import refframe.compiler.compiler.
+
+Local Open Scope Z_scope.
+
+(***
+void gtyield(void)
+{
+	struct gt *old, *new;
+
+	old = &gttbl[gtcur];
+        gtcur = (gtcur+1)%2; // rand()%2;
+	new = &gttbl[gtcur];
+	gtswtch(old, new);
+}
+
+gtswtch.s
+        mov     %rsp, 0x00(%rdi)
+        mov     %r15, 0x08(%rdi)
+        mov     %r14, 0x10(%rdi)
+        mov     %r13, 0x18(%rdi)
+        mov     %r12, 0x20(%rdi)
+        mov     %rbx, 0x28(%rdi)
+        mov     %rbp, 0x30(%rdi)
+
+        mov     0x00(%rsi), %rsp
+        mov     0x08(%rsi), %r15
+        mov     0x10(%rsi), %r14
+        mov     0x18(%rsi), %r13
+        mov     0x20(%rsi), %r12
+        mov     0x28(%rsi), %rbx
+        mov     0x30(%rsi), %rbp
+
+        ret
+***)
+
+Local Coercion ImmediateOp: Z >-> asm_operand.
+Local Coercion RegisterOp: string >-> asm_operand.
+
+
+Definition yield_addr : Z := 2000.
+
+Definition coro_state_addr : Z := 3000.
+
+(*
+Definition yield_asm: gmap Z asm_instr := deep_to_asm_instrs yield_addr
+  [Amov "R9" 0;
+   (** basic setup **)
+   (* R17 := gtcur *)
+   (* Aload "R17" "R9" (gtcur); *)
+   (* R16 := gtnext *)
+   Aslt "R16" "R17" 1;
+
+   (* R15 := gttbl[gtcur] *)
+   Amul "R9" "R17" 13;
+   (* Aadd "R15" "R9" (gttbl); *)
+   (* R14 := gttbl[gtnext] *)
+   Amul "R9" "R16" 13;
+   (* Aadd "R14" "R9" (gttbl); *)
+
+
+   (** store registers to gttbl[gtcur] **)
+   Astore "R19" "R15" 0;
+   Astore "R20" "R15" 1;
+   Astore "R21" "R15" 2;
+   Astore "R22" "R15" 3;
+   Astore "R23" "R15" 4;
+   Astore "R24" "R15" 5;
+   Astore "R25" "R15" 6;
+   Astore "R26" "R15" 7;
+   Astore "R27" "R15" 8;
+   Astore "R28" "R15" 9;
+   Astore "R29" "R15" 10;
+   Astore "R30" "R15" 11;
+   Astore "SP"  "R15" 12;
+
+   (** load gttbl[gtnext] to registers **)
+   Aload "R19" "R14" 0;
+   Aload "R20" "R14" 1;
+   Aload "R21" "R14" 2;
+   Aload "R22" "R14" 3;
+   Aload "R23" "R14" 4;
+   Aload "R24" "R14" 5;
+   Aload "R25" "R14" 6;
+   Aload "R26" "R14" 7;
+   Aload "R27" "R14" 8;
+   Aload "R28" "R14" 9;
+   Aload "R29" "R14" 10;
+   Aload "R30" "R14" 11;
+   Aload "SP"  "R14" 12;
+
+
+   (** argument passing **)
+   (** already handled; argument 0 register == return register == R0 **)
+   (* Amov "R1" "R0"; *)
+   (* Aload "R0" "R9" (yield_val); *)
+   (* Astore "R1" "R9" (yield_val); *)
+
+   Aret]
+.
+*)
+
+Definition coro_saved_regs : list string := "PC"::saved_registers.
+Opaque coro_saved_regs.
+
+Definition yield_swap_reg (r : string) (o : Z) : list deep_asm_instr := [
+    Aload "R17" "R18" o;
+    Astore r "R18" o;
+    Amov r "R17"
+  ].
+
+
+Definition yield_asm: gmap Z asm_instr := deep_to_asm_instrs yield_addr (
+  [Amov "R18" coro_state_addr] ++
+  mjoin (imap (λ i r, yield_swap_reg r (Z.of_nat i)) (locked saved_registers)) ++ [
+  Aload "R17" "R18" (Z.of_nat $ length saved_registers);
+  Astore "R30" "R18" (Z.of_nat $ length saved_registers);
+  Abranch true "R17"]).
+
+Definition coro_get_regs (regs : gmap string Z) : list Z :=
+  ((regs !!!.) <$> coro_saved_regs).
+Arguments coro_get_regs : simpl never.
+
+Definition coro_regs_mem (regs : gmap string Z) : gmap Z (option Z) :=
+  map_seqZ coro_state_addr (Some <$> coro_get_regs regs).
+Arguments coro_regs_mem : simpl never.
+
+Definition coro_regs_regs (regs : gmap string Z) : gmap string Z :=
+  list_to_map ((λ x, (x, regs !!! x)) <$> coro_saved_regs).
+Arguments coro_regs_regs : simpl never.
+
+Lemma coro_regs_regs_lookup_in r rs rs' :
+  r ∈ "PC"::saved_registers →
+  (coro_regs_regs rs ∪ rs') !!! r = rs !!! r.
+Proof.
+Admitted.
+
+Lemma coro_regs_regs_lookup_not_in r rs rs' :
+  r ∉ "PC"::saved_registers →
+  (coro_regs_regs rs ∪ rs') !!! r = rs' !!! r.
+Proof.
+Admitted.
+
+Definition yield_itree : itree (moduleE asm_event (gmap string Z)) unit :=
+  ITree.forever (
+  '(rs, mem) ← TReceive (λ '(rs, mem), (Incoming, EAJump rs mem));;;
+  TAssume (rs !!! "PC" = yield_addr);;;;
+  rsold ← TGet;;;
+  TAssume (coro_regs_mem rsold ⊆ mem);;;;
+  let rs' := (<["PC" := rs !!! "R30"]> rs) in
+  TPut rs';;;;
+  r17 ← TExist Z;;;
+  r18 ← TExist Z;;;
+  TVis (Outgoing, EAJump
+                    (<["R17" := r17]> $ <["R18" := r18]> $ (coro_regs_regs rsold ∪ rs))
+                    (coro_regs_mem rs' ∪ mem))).
+
+Local Ltac go :=
+  clear_itree.
+Local Ltac go_s :=
+  tstep_s; go.
+Local Ltac go_i :=
+  tstep_i; go.
+
+Lemma yield_asm_refines_itree regs :
+  trefines (MS asm_module (initial_asm_state yield_asm))
+           (MS (mod_itree _ _) (yield_itree, regs)).
+Proof.
+  apply: tsim_implies_trefines => n0 /=.
+  unshelve eapply tsim_remember. { simpl. exact (λ _ σa '(t, _),
+    t ≈ yield_itree ∧
+    σa.(asm_cur_instr) = AWaiting ∧
+    σa.(asm_instrs) = yield_asm). }
+  { split!. } { done. }
+  move => n _ Hloop [????] [??] ?. destruct_all?; simplify_eq/=.
+  tstep_i => ????? Hi. simpl.
+  tstep_s. rewrite -/yield_itree. go.
+  go_s. eexists (_, _). go.
+  go_s. split!. go.
+  go_s => ?. go.
+  go_s.
+  go_s => ?. go.
+  go_s.
+  tstep_i => ??. simplify_map_eq'.
+  rewrite /yield_asm deep_to_asm_instrs_cons in Hi. simplify_map_eq.
+  tstep_i.
+  tstep_i. simplify_map_eq'.
+Admitted.
+
+(***
+int
+gtgo(void *f)
+{
+	struct gt *p;
+
+        p = &gttbl[1];
+
+	/* *&stack[StackSize -  8] = (uint64_t)gtstop; */
+	*&stack[StackSize - 16] = (uint64_t)f;
+	p->rsp = (uint64_t)&stack[StackSize - 16];
+
+	return 0;
+}
+***)
+
+(** simply set p->rsp to be stack, p->pc to be the function **)
+(*
+Definition gtgo_addr: Z := 200.
+
+Definition gtgo_asm: gmap Z asm_instr := deep_to_asm_instrs gtgo_addr
+  [
+    Amov "R9" 0;
+    (*** rsp ***)
+    Amov "R10" (stack + stksize);
+    Astore "R10" "R9" (gttbl + 13 + 12);
+
+    (*** PC ***)
+    Astore "R0" "R9" (gttbl + 13 + 11);
+    Aret
+  ]
+.
+*)
+
+
+(***
+void stream_inner(int n) {
+  gtyield_with_val(n);
+  stream_inner(n+1);
+}
+
+void stream()
+{
+  stream_inner(0);
+}
+
+int main(void)
+{
+  gtgo(stream);
+  for(int i=0; i<5; i++) {
+    int v = gtyield_with_val(-1);
+    printf("v is : %d\n", v);
+  }
+}
+***)
+
+Definition stream_addr: Z := 400.
+Definition main_addr: Z := 500.
+Definition print_addr: Z := 600.
+
+Definition stream_imp: fndef := {|
+  fd_args := [("n")];
+  fd_vars := [];
+  fd_body := LetE "_" (imp.Call "yield" [Var "n"]) $
+             (imp.Call "stream" [(BinOp (Var "n") AddOp (Val $ ValNum 1))]);
+  fd_static := I
+|}.
+
+Definition main_imp: fndef := {|
+  fd_args := [];
+  fd_vars := [("x", -1); ("y", -1)];
+  fd_body := LetE "x" (imp.Call "yield" [Val $ ValNum 0]) $
+             LetE "_" (imp.Call "print" [(Var "x")]) $
+             LetE "y" (imp.Call "yield" [Val $ ValNum 0]) $
+             LetE "_" (imp.Call "print" [(Var "y")]) $
+             (Val $ ValNum (-1));
+  fd_static := I
+|}.
+
+Definition all_f2i : gmap string Z :=
+  <["yield"  := yield_addr]> $
+  <["stream" := stream_addr]> $
+  <["main"   := main_addr]> $
+  <["print"  := print_addr]> $
+  ∅.
+
+Definition stream_asm : gmap Z asm_instr :=
+  deep_to_asm_instrs stream_addr ltac:(i2a_compile all_f2i stream_imp).
+
+Definition main_asm : gmap Z asm_instr :=
+  deep_to_asm_instrs main_addr ltac:(i2a_compile all_f2i main_imp).
+
+Lemma stream_asm_refines_imp :
+  trefines (MS asm_module (initial_asm_state stream_asm))
+           (MS (imp_to_asm (dom _ stream_asm) {["stream"]} all_f2i imp_module)
+               (initial_imp_to_asm_state ∅ imp_module (initial_imp_state (<["stream" := stream_imp]> ∅)))).
+Proof.
+  apply: compile_correct; [|done|..].
+  - by vm_compute.
+  - by vm_compute.
+  - move => ??. rewrite /all_f2i !lookup_insert_Some !lookup_empty.
+    move => ?. destruct_all?; simplify_eq; compute_done.
+Qed.
+
+Lemma main_asm_refines_imp :
+  trefines (MS asm_module (initial_asm_state main_asm))
+           (MS (imp_to_asm (dom _ main_asm) {["main"]} all_f2i imp_module)
+               (initial_imp_to_asm_state ∅ imp_module (initial_imp_state (<["main" := main_imp]> ∅)))).
+Proof.
+  apply: compile_correct; [|done|..].
+  - by vm_compute.
+  - by vm_compute.
+  - move => ??. rewrite /all_f2i !lookup_insert_Some !lookup_empty.
+    move => ?. destruct_all?; simplify_eq; compute_done.
+Qed.
+
+Global Instance seq_product_eq_dec : EqDecision seq_product_state.
+Proof. solve_decision. Qed.
+
+Inductive coro_prod_filter_state :=
+| CPFInit (finit : string) (started : bool)
+| CPFLeft
+| CPFRight
+| CPFExited.
+
+Definition coro_prod_filter (fns1 fns2 : gset string) : seq_product_state → coro_prod_filter_state → imp_ev → seq_product_state → coro_prod_filter_state → imp_ev → bool → Prop :=
+  λ p s e p' s' e' ok,
+    match s, p with
+    | CPFInit finit false, SPNone =>
+        ∃ f vs h,
+        e = EICall f vs h ∧
+        e' = e ∧
+        p' = SPLeft ∧
+        ok = bool_decide (f ∈ fns1) ∧
+        s' = CPFInit finit true
+    | CPFInit _ true, SPNone
+    | CPFLeft, SPNone
+    | CPFRight, SPNone =>
+        e' = e ∧
+        p' = (if s is CPFRight then SPRight else SPLeft) ∧
+        s' = s ∧
+        ok = if e is EICall _ _ _ then false else true
+    | CPFInit _ _, _
+    | CPFLeft, _ =>
+        (* p must be SPLeft *)
+        p = SPLeft ∧
+        match e with
+        | EICall f vs h =>
+            if bool_decide (f = "yield") then
+              e' = (if s is CPFInit finit _ then EICall finit vs h else EIReturn (vs !!! 0%nat) h) ∧
+              p' = SPRight ∧
+              s' = CPFRight ∧
+              ok = bool_decide (length vs = 1%nat)
+            else
+              e' = e ∧
+              p' = (if bool_decide (f ∈ fns2) then SPRight else SPNone) ∧
+              s' = s ∧
+              ok = bool_decide (f ∉ fns2)
+        | EIReturn v h =>
+            e' = e ∧
+            p' = SPNone ∧
+            s' = CPFExited ∧
+            ok = true
+        end
+    | CPFRight, _ =>
+        (* p must be SPRight: Not *)
+        p = SPRight ∧
+        match e with
+        | EICall f vs h =>
+            if bool_decide (f = "yield") then
+              e' = EIReturn (vs !!! 0%nat) h ∧
+              p' = SPLeft ∧
+              s' = CPFLeft ∧
+              ok = bool_decide (length vs = 1%nat)
+            else
+              e' = e ∧
+              p' = SPNone ∧
+              s' = s ∧
+              ok = bool_decide (f ∉ fns1)
+        | EIReturn v h =>
+            ok = false
+        end
+    | CPFExited, _ =>
+        ok = false
+    end.
+Arguments coro_prod_filter _ _ _ _ _ _ _ _ /.
+
+Definition coro_prod (fns1 fns2 : gset string) (m1 m2 : module imp_event) : module imp_event :=
+  mod_link (coro_prod_filter fns1 fns2) m1 m2.
+
+Definition initial_coro_prod_state (finit : string) (m1 m2 : module imp_event) (σ1 : m1.(m_state)) (σ2 : m2.(m_state)) :=
+  (@MLFNone imp_ev, CPFInit finit false, σ1, σ2).
+
+Lemma coro_prod_trefines m1 m1' m2 m2' σ1 σ1' σ2 σ2' σ ins1 ins2 `{!VisNoAll m1} `{!VisNoAll m2}:
+  trefines (MS m1 σ1) (MS m1' σ1') →
+  trefines (MS m2 σ2) (MS m2' σ2') →
+  trefines (MS (coro_prod ins1 ins2 m1 m2) (σ, σ1, σ2))
+           (MS (coro_prod ins1 ins2 m1' m2') (σ, σ1', σ2')).
+Proof. move => ??. by apply mod_link_trefines. Qed.
+
+Definition yield_asm_dom : gset Z := locked (dom _) yield_asm.
+
+Definition initial_asm_prod_state (m1 m2 : module asm_event) (σ1 : m1.(m_state)) (σ2 : m2.(m_state)) :=
+  (@MLFNone asm_ev, @None seq_product_state, σ1, σ2).
+
+(* Definition coro_spec_inv m1 m2 *)
+(*   (σ1 : (asm_prod yield_asm_dom ∅ asm_module (imp_to_asm ∅ ∅ ∅ (imp_prod ∅ ∅  m1 m2))).(m_state)) *)
+(*   (σ2 : (imp_to_asm ∅ ∅ ∅ (coro_prod ∅ ∅ m1 m2)).(m_state)) : Prop := *)
+(*   let '(σa, σap, (AsmState i _ _ yins) , (σsm, (σi, cs, σi1, σi2), _)) := σ1 in *)
+(*   yins = yield_asm ∧ *)
+(*   i *)
+(*   . *)
+(*   → mod_link_state asm_ev * option seq_product_state * asm_state * *)
+(*     (mod_seq_map_state imp_event * (mod_link_state imp_ev * list seq_product_state * m_state m1 * m_state m2) * *)
+(*      (pp_state * imp_to_asm_state * uPred imp_to_asmUR)) *)
+(*     → mod_seq_map_state imp_event * (mod_link_state imp_ev * bool * m_state m1 * m_state m2) * *)
+(*       (pp_state * imp_to_asm_state * uPred imp_to_asmUR) → Prop *)
+
+
+  (* let 'Imp e1 h1 fns1' := σ1 in *)
+  (* let '(σf, cs, Imp el hl fnsl, Imp er hr fnsr) := σ2 in *)
+  (* ∃ n K Kl Kr e1' el' er' bl br, *)
+  (* fns1' = fns1 ∪ fns2 ∧ *)
+  (* fnsl = fns1 ∧ *)
+  (* fnsr = fns2 ∧ *)
+  (* imp_link_prod_combine_ectx n bl br σf cs K Kl Kr ∧ *)
+  (* e1 = expr_fill K e1' ∧ *)
+  (* el = expr_fill Kl el' ∧ *)
+  (* er = expr_fill Kr er' ∧ *)
+  (* match σf with *)
+  (* | MLFLeft => e1' = el' ∧ is_static_expr true el' ∧ er' = Waiting br ∧ h1 = hl *)
+  (*             ∧ (if bv then to_val el' = None else True) *)
+  (* | MLFRight => e1' = er' ∧ is_static_expr true er' ∧ el' = Waiting bl ∧ h1 = hr *)
+  (*              ∧ (if bv then to_val er' = None else True) *)
+  (* | MLFNone => e1' = Waiting (bl || br) ∧ el' = Waiting bl ∧ er' = Waiting br *)
+  (* | _ => False *)
+  (* end. *)
+
+Lemma i2a_mem_lookup_big sp gp m mem :
+  i2a_mem_inv sp gp mem -∗
+  i2a_mem_map m -∗
+  ⌜m ⊆ mem⌝.
+Proof.
+  iDestruct 1 as (Hsp) "(?&?&Hauth)".
+  iIntros "Hconst".
+  by iDestruct (i2a_mem_lookup_big' with "Hauth Hconst") as %?.
+Qed.
+
+
+(* We cannot use this lemma with imp_to_asm_combine since yield is not
+part of fns but parts of ins, but maybe we don't care? *)
+Theorem coro_spec m1 m2 σ1 σ2 ins1 ins2 fns1 fns2 f2i1 f2i2 finit regs_init
+  `{!VisNoAll m1} `{!VisNoAll m2}:
+  let fns := {["yield"]} ∪ fns1 ∪ fns2 in
+  let ins := yield_asm_dom ∪ ins1 ∪ ins2 in
+  let f2i := f2i1 ∪ f2i2 in
+  f2i2 !! finit = Some (regs_init !!! "PC") →
+  finit ∈ fns2 →
+  "yield" ∉ fns1 ∪ fns2 →
+  ins1 ## ins2 →
+  fns1 ## fns2 →
+  yield_asm_dom ## ins1 ∪ ins2 →
+  f2i1 !! "yield" = Some yield_addr →
+  f2i2 !! "yield" = Some yield_addr →
+  (∀ f, f ∈ fns1 → ∃ i, i ∈ ins1 ∧ f2i1 !! f = Some i) →
+  (∀ f, f ∈ fns2 → ∃ i, i ∈ ins2 ∧ f2i2 !! f = Some i) →
+  (∀ f i1 i2, f2i1 !! f = Some i1 → f2i2 !! f = Some i2 → i1 = i2) →
+  (∀ f i, f2i1 !! f = Some i → i ∈ ins2 → f ∈ fns2) →
+  (∀ f i, f2i2 !! f = Some i → i ∈ ins1 → f ∈ fns1) →
+  trefines
+    (MS (asm_prod yield_asm_dom (ins1 ∪ ins2) asm_module
+           (asm_prod ins1 ins2 (imp_to_asm ins1 fns1 f2i1 m1) (imp_to_asm ins2 fns2 f2i2 m2)) )
+        (initial_asm_prod_state asm_module (asm_prod _ _ _ _)
+           (initial_asm_state yield_asm)
+           (initial_asm_prod_state (imp_to_asm _ _ _ _) (imp_to_asm _ _ _ _)
+              (initial_imp_to_asm_state ∅ m1 σ1)
+              (initial_imp_to_asm_state ∅ m2 σ2))))
+    (MS (imp_to_asm ins fns f2i (coro_prod fns1 fns2 m1 m2))
+       (initial_imp_to_asm_state (coro_regs_mem regs_init) (coro_prod _ _ _ _)
+          (initial_coro_prod_state finit _ _ σ1 σ2)))
+.
+Proof.
+  move => fns ins f2i Hinit Hfinit Hyf Hidisj Hfdisj Hydisj Hy1 Hy2 Hi1 Hi2 Hag Hf1 Hf2.
+  have ? : ∀ f i1 i2, f2i1 !! f  = Some i1 → f2i !! f = Some i2 → i1 = i2. admit.
+  etrans. { apply: asm_prod_trefines; [|done]. apply (yield_asm_refines_itree regs_init). }
+  apply: tsim_implies_trefines => n0 /=.
+  tstep_i => *. case_match; destruct_all?; simplify_eq/=.
+  tstep_s. split!.
+  tstep_s. move => -[] //= ? h gp vs avs ret f *.
+  tstep_s. split!.
+  tstep_s => ?.
+  have ? : regs !!! "PC" ∈ ins1. { efeed pose proof Hi1; [done|]. destruct_all?. simplify_eq. naive_solver. }
+  rewrite bool_decide_false; [|set_solver].
+  rewrite bool_decide_true; [|set_solver].
+  tstep_i => *. case_match; destruct_all?; simplify_eq/=.
+  rewrite bool_decide_true; [|set_solver].
+  tstep_i => *. simplify_eq.
+  tstep_i. eexists true. split; [done|]. eexists h, gp, vs, avs, ret, f.
+  split!. { admit. (* naive_solver. *) } { set_solver. }
+  { iSatMono. iIntros!. iFrame. iSplitR; [|iAccu]. by iApply big_sepM_empty. }
+  tsim_mirror m1 σ1. move => ??? Hcont.
+  tstep_both. apply Hcont => κ ?? Hs. destruct κ.
+  2: { tstep_s. eexists None. apply: steps_spec_step_end; [done|] => ??. tend. split!; [done|]. eauto. }
+  clear Hcont Hs. move => ?. subst.
+  tstep_s. eexists (Some (Incoming, _)). split!. apply: steps_spec_step_end; [done|] => ??. tend. split!; [done|].
+  unshelve apply: tsim_remember. { simpl. exact (λ _
+      '(σpy1, σpy2, (yt, yregs), (σpc1, σpc2, (σsm1, σ1, (pp1, (I2A cs1 lr1), x1)), (σsm2, σ2, (pp2, (I2A cs2 lr2), x2))))
+      '(σsm', (σlc, σc, σ1', σ2'), (ppc, (I2A csc lrc), xc)),
+       ∃ cret cgp cregs,
+       eqit eq true false yt yield_itree ∧
+       σ1' = σ1 ∧
+       σ2' = σ2 ∧
+       σpy1 = MLFRight ∧
+       σpy2 = None ∧
+       σpc2 = None ∧
+       σsm' = SMProg ∧
+       ppc = PPInside ∧
+       csc = [I2AI false cret cgp cregs] ∧
+       cret ∉ ins ∧
+       match σc with
+       (* Left side, not yet changed to right side *)
+       | CPFInit finit started =>
+           started = true ∧
+           σpc1 = MLFLeft ∧
+           σsm1 = SMProg ∧
+           pp1 = PPInside ∧
+           cs1 = csc ∧
+           lrc = lr1 ∧
+           x1 = (i2a_mem_map (coro_regs_mem yregs) ∗ xc)%I ∧
+           σsm2 = SMFilter ∧
+           pp2 = PPOutside ∧
+           cs2 = [] ∧
+           lr2 = ∅ ∧
+           (x2 ⊣⊢ emp)%I ∧
+           σlc = MLFLeft ∧
+           f2i2 !! finit = Some (yregs !!! "PC") ∧
+           finit ∈ fns2
+       (* Left side, already changed to right side *)
+       | CPFLeft => False
+       (* Right side *)
+       | CPFRight => False
+       (* returned from left side *)
+       (* | 3%nat => False *)
+       | _ => False
+       end). }
+  { split!. apply big_sepM_empty. } { done. }
+  clear -Hyf Hidisj Hfdisj Hydisj Hy1 Hy2 Hi1 Hi2 Hag Hf1 Hf2 VisNoAll0 VisNoAll1.
+  move => n ? Hloop [[[σpy1 σpy2][yt yregs]][[[σpc1 σpc2][[σsm1 σ1][[pp1 [cs1 lr1]]x1]]][[σsm2 σ2][[pp2 [cs2 lr2]]x2]]]].
+  move => [[σsm' [[[σlc σc] σ1'] σ2']][[ppc [csc lrc]] xc]] [state ?]. destruct_all?; simplify_eq.
+  destruct σc as [finit| | |] => //; destruct_all?; simplify_eq.
+  - tsim_mirror m1 σ1. move => ??? Hcont.
+    tstep_both. apply Hcont => κ ? Hstep Hs. destruct κ as [[? e]|].
+    2: { tstep_s. eexists None. apply: steps_spec_step_end; [done|] => ??. tend. split!; [done|]. eauto. }
+    clear Hcont Hs.
+    tend. have [σ' Hσ'] := vis_no_all _ _ _ Hstep. eexists σ'. split; [naive_solver|].
+    destruct i; [by tstep_i|].
+    tstep_s. eexists (Some (Outgoing, e)).
+    destruct e => /=; [case_bool_decide|]; split!.
+    all: apply: steps_spec_step_end; [done|] => σ'' ?; assert (σ'' = σ') by naive_solver.
+    + (* left to right *)
+      tstep_s => ?.
+      tstep_i => *. destruct_all?; simplify_map_eq'.
+      rewrite bool_decide_false. 2: set_solver.
+      rewrite bool_decide_false. 2: admit. (* 2: set_solver. *)
+      move => /= *. destruct_all?; simplify_map_eq'.
+      rewrite bool_decide_true. 2: rewrite /yield_asm_dom; unlock; admit.
+      tstep_i. rewrite -/yield_itree. go.
+      go_i => -[??]. go.
+      go_i => ?. simplify_eq. go.
+      go_i. split; [done|]. go.
+      go_i.
+      iSatStart. iIntros!.
+      iDestruct (i2a_mem_lookup_big with "[$] [$]") as %?.
+      iSatStop.
+      go_i. split!. go.
+      go_i.
+      go_i => ?. go.
+      go_i => ?. go.
+      go_i => *. destruct_all?. simplify_map_eq'. go.
+      rewrite (coro_regs_regs_lookup_in "PC"); [|compute_done].
+      rewrite bool_decide_false. 2: admit.
+      rewrite bool_decide_true. 2: admit.
+      tstep_i => *. destruct_all?; simplify_eq/=. destruct_all?; simplify_map_eq'.
+      rewrite (coro_regs_regs_lookup_in "PC"); [|compute_done].
+      rewrite bool_decide_false. 2: admit.
+      rewrite bool_decide_true. 2: admit.
+      tstep_i => *. simplify_eq.
+      tstep_i. eexists true. split!.
+      { admit. } { done. }
+      { simplify_map_eq'. rewrite (coro_regs_regs_lookup_in "PC"); [|compute_done]. done. }
+      { admit. } { rewrite /i2a_regs_call. simplify_map_eq'. apply (coro_regs_regs_lookup_not_in "R30"). compute_done. }
+      { iSatMono. setoid_subst. iFrame. admit. }
+
+      admit.
+    + (* left call to outside *)
+      case_bool_decide; [by tstep_s|].
+      rewrite bool_decide_true //=.
+      tstep_i => *. destruct_all?; simplify_eq.
+      rewrite bool_decide_false. 2: admit.
+      rewrite bool_decide_false. 2: admit.
+      move => /= *. destruct_all?; simplify_eq/=.
+      rewrite bool_decide_false. 2: admit.
+      rewrite bool_decide_false. 2: admit.
+      tstep_s. split!. done. set_solver. admit. 2: done. set_solver.
+      { iSatMono. iIntros!. iFrame. iAccu. }
+      iSatClear.
+
+      (* go back inside *)
+      tstep_i => e *. destruct e; destruct_all?; simplify_eq.
+      tstep_s. split!.
+      tstep_s => -[] /= *. { tstep_s. split!. by tstep_s. }
+      tstep_s. split!. destruct_all?; simplify_eq.
+      rewrite bool_decide_false. 2: admit.
+      rewrite bool_decide_true. 2: set_solver.
+      tstep_i => /= *. destruct_all?; simplify_eq/=. destruct_all?; simplify_eq/=.
+      rewrite bool_decide_true; [|done].
+      tstep_i => *. simplify_eq.
+      tstep_i => *. eexists false. split!. done.
+      { iSatMono. iIntros!. iFrame. iAccu. }
+      tsim_mirror m1 σ' => ??? Hcont.
+      tstep_both. apply Hcont => -[?|] ?? Hs *. simplify_eq.
+      2: { tstep_s. eexists None. apply: steps_spec_step_end; [done|] => ??. tend. split!; [done|]. eauto. }
+      tstep_s. eexists (Some (Incoming, _)). split!.
+      apply: steps_spec_step_end; [done|] => ??. tend. split!; [done|].
+      apply: Hloop. { etrans; [|done]. etrans; [|done]. apply ti_le_S. }
+      split!.
+    + (* left return to outside *)
+      tstep_i => *. destruct_all?; simplify_eq.
+      rewrite bool_decide_false. 2: set_solver.
+      rewrite bool_decide_false. 2: set_solver.
+      move => /= *. destruct_all?; simplify_eq/=.
+      rewrite bool_decide_false. 2: set_solver.
+      rewrite bool_decide_false. 2: set_solver.
+      tstep_s. split!. done.
+      { iSatMono. iIntros!. iFrame. iAccu. }
+      iSatClear.
+
+      (* going back inside leads to UB *)
+      tstep_i => e *. tstep_s. split!.  destruct_all?; simplify_eq/=.
+      destruct e; destruct_all?; simplify_eq.  tstep_s => -[] /= *; tstep_s; split!; by tstep_s.
+Abort.
